CCodeGen added

Verse/Arch/C.v
@@ -10,10 +10,53 @@ Require Import Error.
 Require Import PrettyPrint.
 
 Require Import List.
+Import ListNotations.
 Require Import String.
 Require Import Ensembles.
 Require Import Program.Basics.
 
+Set Implicit Arguments.
+
+Module CP.
+
+  Definition void : Doc                    := text "void".
+  Definition uint_t   (n : nat)            := text "uint" <> decimal n <> text "_t".
+  Definition statements (x : list Doc) : Doc := sepBy (text ";" <> line) x <> text ";".
+  Definition body b := brace (nest 4 (line <> b) <> line).
+  Definition while c b := text "while" <> c <> line <> body b.
+  Definition voidFunction (nm : string)
+             (args bdy : list Doc)
+    := void <_> text nm <> paren (commaSep args) <> line <> body (statements bdy).
+  
+  Definition register (decl : Doc) := text "register" <_> decl.
+  Definition deref    v            := paren (text "*" <> v).
+  Definition assign   x y          := x <_> text "=" <_> y.
+  Definition plusplus d            := text "++" <> d.
+  Definition minusminus d          := text "--" <> d.
+                                                     
+End CP.
+
+
+Inductive creg : varT :=
+  cr (ty : type) : string -> creg ty.
+
+Inductive cvar : varT :=
+| inRegister (ty : type) : creg ty -> cvar ty
+| onStack    (ty : type) : string -> cvar ty
+.
+
+Instance cRegPretty : forall ty, PrettyPrint (creg ty)
+  := { doc := fun x => match x with
+                       | cr _ n => text "r_" <> text n
+                       end
+     }.
+
+Instance cMachineVar : forall ty, PrettyPrint (cvar ty)
+  := { doc := fun x => match x with
+                       | inRegister r => doc r
+                       | onStack _  s => text s
+                       end
+     }.
 
 Module C <: ARCH.
 
@@ -23,17 +66,11 @@ Module C <: ARCH.
 
   (** The registers for this architecture *)
 
-  Inductive creg : varT :=
-    cr (ty : type) : string -> creg ty.
-
-  Inductive cvar : varT :=
-  | inRegister (ty : type) : creg ty -> cvar ty
-  | onStack    (ty : type) : string -> cvar ty
-  .
-
   Definition register := creg.
 
   Definition machineVar := cvar.
+
+  Definition Word := Word64.
 
   Definition embedRegister := inRegister.
 
@@ -65,26 +102,34 @@ Module CFrame <: FRAME C.
   
   Definition frameState := C.frameDescription.
 
+  Definition emptyFrame (s : string) : frameState.
+    refine (
+        let fv := {| fname := s; param := []; local := [] |} in
+        existT _ fv _
+      ).
+    constructor; simpl; constructor.
+    Defined.
+    
   Definition addParam (ty : type) (a : machineVar ty) (f : frameState) : frameState.
     refine (
-  existT _ {| param := ty :: param (projT1 f); local := local (projT1 f) |} {| pa := _; la := _ |}
+  existT _ {| fname := fname (projT1 f); param := ty :: param (projT1 f); local := local (projT1 f) |} {| pa := _; la := _ |}
       ).
     simpl.
-    exact ((a, pa _ (projT2 f))).
-    exact (la _ (projT2 f)).
+    exact ((a, pa (projT2 f))).
+    exact (la (projT2 f)).
+    
   Defined.
 
   Definition addLocal (ty : type) (a : machineVar ty) (f : frameState) : frameState.
     refine (
-        existT _ {| param := param (projT1 f); local := ty :: local (projT1 f) |} {| pa := _; la := _ |}
+        existT _ {| fname := fname (projT1 f); param := param (projT1 f); local := ty :: local (projT1 f) |} {| pa := _; la := _ |}
       ).
     simpl.
-    exact (pa _ (projT2 f)).
-    exact ((a, la _ (projT2 f))).
+    exact (pa (projT2 f)).
+    exact ((a, la (projT2 f))).
   Defined.
   
-
-  Definition paramAlloc (f : frameState) (ty : type) : frameState + { not (In _ supportedType ty) }.
+  Definition paramAlloc (f : frameState) (ty : type) : (machineVar ty) * frameState + { not (In _ supportedType ty) }.
     refine (
     let n := List.length (param (projT1 f)) in
     match ty with
@@ -93,16 +138,18 @@ Module CFrame <: FRAME C.
     | word 2
 
     | word 3
-    | array _ _ _ => inleft (addParam ty (onStack _ ("l_" ++ Internal.nat_to_str n)) f)
+    | array _ _ _ => let v := onStack ty ("l_" ++ Internal.nat_to_str n)%string in
+                                      inleft (v, addParam v f)
     | _           => inright _
     end
       ).
+    
     all : unfold In;
       unfold supportedType;
-      unfold not; intros; inversion H.
+      unfold not; intro H; inversion H.
     Defined.
 
-    Definition onStack (f : frameState) (ty : type) : frameState + { not (In _ supportedType ty) }.
+    Definition onStack (f : frameState) (ty : type) : (machineVar ty) * frameState + { not (In _ supportedType ty) }.
       refine (
     let n := List.length (param (projT1 f)) in
     match ty with
@@ -110,7 +157,8 @@ Module CFrame <: FRAME C.
     | word 1 
     | word 2
     | word 3
-    | array _ _ _ => inleft (addLocal ty (onStack _ ("l_" ++ Internal.nat_to_str n)) f)
+    | array _ _ _ => let v := onStack ty ("l_" ++ Internal.nat_to_str n) in
+                     inleft (v, addLocal v f)
     | _           => inright _
     end
         ).
@@ -119,7 +167,7 @@ Module CFrame <: FRAME C.
         unfold not; intro H; inversion H.
     Defined.
       
-    Definition useRegister (ty : type) (f : frameState) (r : register ty) : frameState + { not (In _ supportedType ty) }.
+    Definition useRegister (ty : type) (f : frameState) (r : register ty) : (machineVar ty) * frameState + { not (In _ supportedType ty) }.
       refine (
           let n := List.length (param (projT1 f)) in
           match ty with
@@ -128,7 +176,8 @@ Module CFrame <: FRAME C.
           | word 2
 
           | word 3
-          | array _ _ _ => inleft (addLocal ty (inRegister _ r) f)
+          | array _ _ _ => let v := inRegister r in
+                           inleft (v, addLocal v f)
           | _           => inright _
           end
         ).
@@ -141,3 +190,55 @@ Module CFrame <: FRAME C.
     Definition description : frameState -> frameDescription := id.
 
 End CFrame.
+
+Module CCodeGen <: CODEGEN C.
+
+  Import C.
+
+  Definition emit (i : instruction (machineVar)) : Doc + { not (supportedInst i) } :=
+    inleft (doc i).
+
+  Local Definition type_doc (t : type) := text (
+                                              match t with
+                                              | word 0 => "uint8_t"%string
+                                              | word 1 => "uint16_t"%string
+                                              | word 2 => "uint32_t"%string
+                                              | word 3 => "uint64_t"%string
+                                              | _      => ""%string
+                                              end).
+
+  Local Definition declareArray (a : Doc)(n : nat) (ty : type) := type_doc ty  <_> a <> bracket (decimal n).
+
+  Definition declare {varty : type}(v : machineVar varty) : Doc :=
+    let vDoc := doc v in
+    match varty with
+    | @Internal.array n _ ty => declareArray vDoc n ty
+    | _                      => type_doc varty <_> vDoc
+    end.
+
+  Fixpoint alloc_declare (l : list type) : forall a : allocation machineVar l, list Doc :=
+    match l with
+    | []        => fun _ => []
+    | (t :: lt) => fun a : allocation machineVar (t :: lt) => declare (fst a) :: (alloc_declare lt (snd a))
+    end.
+
+  Definition prologue (f : frameDescription) : Doc :=
+    let 'existT _ fv fa := f in
+    let localDec := alloc_declare (local fv) (la fa) in
+    let paramDec := alloc_declare (param fv) (pa fa) in
+    lineSep [ text "#include <stdint.h>" ;
+                CP.voidFunction (fname fv) paramDec
+                                localDec
+            ].
+
+  Definition epilogue : frameDescription -> Doc := fun _ => NilDoc.
+
+  Definition loopWrapper (msgTy : type) (v : machineVar msgTy) (n : machineVar Word) (d : Doc) : Doc :=
+    let loopCond := paren (doc n <_> text "> 0") in
+    CP.while loopCond
+             (
+               d <> CP.statements [ CP.plusplus (doc v) ;  CP.minusminus (doc n) ]
+             ).
+
+End CCodeGen.
+
